Fix delocation by requiring definedness for additional parameters.
This is a fix for now, but it breaks the nice untyped setup we had
before the change of the environments from env to onv.
The problem is that additional paramters induce reads  function
applications -- which might get stuck now. In the old setup a variable
read could never get stuck.

There is an interesting relation between liveness and this problem. If
only live variables are added as additional parameters, it might look
like we can get around the definedness requirement, as any live variable
is guaranteed to be read later anyway. However, in the presence of
syscalls this is not true: the read may occur only after a syscall, i.e.
the translated program will crash before issuing the syscall -- and
hence is not equivalent.

Delocation.v
@@ -1,4 +1,4 @@
-Require Import AllInRel Util Map Env EnvTy Exp IL Annotation Coherence Bisim DecSolve Liveness Restrict.
+Require Import AllInRel Util Map Env EnvTy Exp IL Annotation Coherence Bisim DecSolve Liveness Restrict MoreExp.
 
 (*  IL_Types. *)
 
@@ -59,15 +59,18 @@ Fixpoint compile (ZL:list (list var)) (s:stmt) (an:ann (list var)) : stmt :=
   end.
 
 Inductive approx
-  : list (option (set var)) -> list (params) -> I.block -> I.block -> Prop :=
-  blk_approxI o (Za Z':list var) DL ZL s ans ans_lv
-  (RD:forall G, o = Some G ->
-                trs (restrict (Some G::DL) G) (Za::ZL) s ans_lv ans)
-  : approx (o::DL) (Za::ZL)(I.blockI Z' s) (I.blockI (Z'++Za) (compile (Za::ZL) s ans)).
+  : list (set var * list var)
+    -> list (option (set var))
+    -> list (params) -> I.block -> I.block -> Prop :=
+  blk_approxI o (Za Z':list var) DL ZL Lv s ans ans_lv ans_lv'
+              (RD:forall G, o = Some G ->
+                       live_sound ((getAnn ans_lv',Z'++Za)::Lv) (compile (Za :: ZL) s ans) ans_lv'
+                       /\ trs (restrict (Some G::DL) G) (Za::ZL) s ans_lv ans)
+  : approx ((getAnn ans_lv',Z'++Za)::Lv) (o::DL) (Za::ZL) (I.blockI Z' s) (I.blockI (Z'++Za) (compile (Za::ZL) s ans)).
 
-Lemma approx_restrict DL ZL L L' G
-: AIR4 approx DL ZL L L'
-  -> AIR4 approx (restrict DL G) ZL L L'.
+Lemma approx_restrict Lv DL ZL L L' G
+: AIR53 approx Lv DL ZL L L'
+  -> AIR53 approx Lv (restrict DL G) ZL L L'.
 Proof.
   intros. general induction H.
   + econstructor.
@@ -76,68 +79,142 @@ Proof.
       rewrite <- restrict_incl; eauto. rewrite restrict_idem; eauto.
 Qed.
 
+Definition appsnd {X} {Y} (s:X * list Y) (t: list Y) := (fst s, snd s ++ t).
+
+Definition defined_on {X} `{OrderedType X} {Y} (G:set X) (E:X -> option Y)
+  := forall x, x ∈ G -> exists y, E x = Some y.
+
+Lemma defined_on_update_some X `{OrderedType X} Y (G:set X) (E:X -> option Y) x v
+  : defined_on (G \ {{x}}) E
+    -> defined_on G (E [x <- Some v]).
+Proof.
+  unfold defined_on; intros. lud.
+  - eauto.
+  - eapply H0; eauto. cset_tac; intuition.
+Qed.
+
+Lemma defined_on_incl X `{OrderedType X} Y (G G':set X) (E:X -> option Y)
+  : defined_on G E
+    -> G' ⊆ G
+    -> defined_on G' E.
+Proof.
+  unfold defined_on; intros; eauto.
+Qed.
+
 Inductive trsR : I.state -> I.state -> Prop :=
-  trsRI (E E':onv val) L L' s ans ans_lv DL ZL
+  trsRI (E E':onv val) L L' s ans Lv' ans_lv ans_lv' DL ZL
   (RD: trs DL ZL s ans_lv ans)
-  (EA: AIR4 approx DL ZL L L')
-  (EQ: E ≡ E')
+  (EA: AIR53 approx Lv' DL ZL L L')
+  (EQ: (@feq _ _ eq) E E')
+  (LV': live_sound Lv' (compile ZL s ans) ans_lv')
+  (EDEF: defined_on (getAnn ans_lv') E')
   : trsR (L, E, s) (L', E', compile ZL s ans).
 
+Lemma omap_var_defined_on Za lv E
+: of_list Za ⊆ lv
+  -> defined_on lv E
+  -> exists l, omap (exp_eval E) (List.map Var Za) = Some l.
+Proof.
+  intros. general induction Za; simpl.
+  - eauto.
+  - simpl in *.
+    edestruct H0.
+    + instantiate (1:=a). cset_tac; intuition.
+    + rewrite H1; simpl. edestruct IHZa; eauto.
+      cset_tac; intuition.
+      rewrite H2; simpl. eauto.
+Qed.
+
+Lemma defined_on_update_list lv (E:onv val) Z vl
+: length vl = length Z
+  -> defined_on (lv \ of_list Z) E
+  -> defined_on lv (E [Z <-- List.map Some vl]).
+Proof.
+  unfold defined_on; intros.
+  decide (x ∈ of_list Z).
+  - eapply length_length_eq in H. clear H0.
+    general induction H; simpl in * |- *.
+    + exfalso. cset_tac; intuition.
+    + lud; eauto. edestruct IHlength_eq; eauto. cset_tac; intuition.
+  - edestruct H0; eauto. instantiate (1:=x). cset_tac; intuition.
+    exists x0. rewrite <- H2.
+    eapply update_with_list_no_update; eauto.
+Qed.
+
+
+
 Lemma trsR_sim σ1 σ2
-  : trsR σ1 σ2 -> sim σ1 σ2.
+  : trsR σ1 σ2 -> bisim σ1 σ2.
 Proof.
   revert σ1 σ2. cofix; intros.
-  intros. destruct H; inv RD; simpl; try provide_invariants_4.
-  + case_eq (exp_eval E e); intros.
-    econstructor; eauto using I.step, plus.
-    rewrite EQ in H0; econstructor; eauto using I.step, plus.
-    eapply trsR_sim. econstructor; eauto using approx_restrict.
-    rewrite EQ; reflexivity.
-    eapply simE; try eapply star_refl; eauto; stuck. rewrite EQ in H0; congruence.
-
-  + case_eq (exp_eval E e); intros.
+  intros. destruct H; inv RD; invt live_sound; simpl; try provide_invariants_53.
+  - remember (exp_eval E e). symmetry in Heqo.
+    pose proof Heqo. rewrite EQ in H0.
+    destruct o.
+    + one_step. simpl in *.
+      eapply trsR_sim.
+      econstructor; eauto using approx_restrict.
+      rewrite EQ; reflexivity.
+      eapply defined_on_update_some. eapply defined_on_incl; eauto.
+    + no_step.
+  - remember (exp_eval E e). symmetry in Heqo.
+    pose proof Heqo. rewrite EQ in H1.
+    destruct o.
     case_eq (val2bool v); intros.
-    one_step. rewrite <- EQ; eauto.
-    eapply trsR_sim; econstructor; eauto.
-    one_step. rewrite <- EQ; eauto.
-    eapply trsR_sim; econstructor; eauto.
-    no_step; rewrite <- EQ in def; congruence.
-  + no_step. simpl. rewrite EQ; eauto.
-  + simpl counted in *.
+    + one_step. eapply trsR_sim; econstructor; eauto using defined_on_incl.
+    + one_step. eapply trsR_sim; econstructor; eauto using defined_on_incl.
+    + no_step.
+  - no_step. simpl. rewrite EQ; eauto.
+  - simpl counted in *.
     decide (length Z' = length Y).
     case_eq (omap (exp_eval E) Y); intros.
-    one_step. simpl in *; eauto.
-    repeat rewrite app_length.
-    eapply get_drop_eq in H6; eauto. inv H6; subst. simpl.
-    rewrite map_length.
-    erewrite get_nth_default; eauto.
-    rewrite <- H5, <- H6 in EA1.
-    eapply omap_exp_eval_app. erewrite omap_agree; eauto.
-    intros. rewrite EQ. reflexivity.
-    eapply trsR_sim; econstructor; eauto using approx_restrict.
-    eapply approx_restrict. rewrite H6, H5. eauto.
-
-    eapply get_drop_eq in H6; eauto. inv H6. simpl.
-    rewrite update_with_list_app.
-    erewrite get_nth_default; eauto.
-    rewrite update_with_list_lookup_list. rewrite EQ. reflexivity.
-    intuition.
-    edestruct (AIR4_length); eauto; dcr.
-    exploit omap_length; eauto. congruence.
-    no_step. get_functional; subst. simpl in *.
-    rewrite omap_app in def.
-    erewrite omap_agree in H7. Focus 2.
-    intros. rewrite EQ. reflexivity. rewrite H7 in def. simpl in *. congruence.
-    no_step.
-    get_functional; subst. simpl in *. congruence.
-    get_functional; subst. simpl in *.
-    apply n. repeat rewrite app_length in len.
-    eapply get_drop_eq in H6; eauto. subst Za0.
-    erewrite get_nth_default in len; eauto. rewrite map_length in len. omega.
-  + one_step.
+    simpl in *.
+    erewrite get_nth_default in H9; eauto.
+    edestruct (omap_var_defined_on x); eauto.
+    eapply get_in_incl; intros.
+    exploit H9. eapply get_app_right. Focus 2.
+    eapply map_get_1; eauto. reflexivity. inv X. eauto.
+    + exploit get_drop_eq; try eapply H11; eauto. subst o.
+      exploit get_drop_eq; try eapply H12; eauto. subst x.
+      erewrite get_nth_default; eauto.
+      one_step.
+      * simpl; eauto.
+        repeat rewrite app_length.
+        rewrite map_length; eauto.
+      * instantiate (1:=l ++ x0).
+        rewrite omap_app.
+        erewrite omap_agree. Focus 2.
+        intros. rewrite <- EQ. reflexivity.
+        rewrite H0; simpl. rewrite H8; simpl. reflexivity.
+      * exploit RD0; eauto; dcr. simpl.
+        eapply trsR_sim; econstructor; eauto.
+        rewrite <- H11, <- H10, <- H12 in EA1.
+        eapply (approx_restrict G' EA1).
+        simpl. rewrite map_app.
+        rewrite update_with_list_app.
+        rewrite (omap_self_update E' Za0). rewrite EQ. reflexivity. eauto.
+        rewrite map_length.
+        exploit omap_length; try eapply H0; eauto. congruence.
+        eapply defined_on_update_list; eauto using defined_on_incl.
+        exploit omap_length; try eapply H0; eauto.
+        exploit omap_length; try eapply H8; eauto.
+        rewrite map_length in X0.
+        repeat rewrite app_length. omega.
+    + no_step. get_functional; subst. simpl in *.
+      rewrite omap_app in def.
+      erewrite omap_agree in H0. Focus 2.
+      intros. rewrite EQ. reflexivity. rewrite H0 in def. simpl in *. congruence.
+    + no_step.
+      get_functional; subst. simpl in *. congruence.
+      get_functional; subst. simpl in *.
+      apply n. repeat rewrite app_length in len.
+      eapply get_drop_eq in H12; eauto. subst Za0.
+      erewrite get_nth_default in len; eauto. rewrite map_length in len. omega.
+  - one_step.
     eapply trsR_sim; econstructor; eauto.
     econstructor; eauto. econstructor.
-    intros. inv H1. eauto.
+    intros. split; eauto. inv H1. eauto.
+    eauto using defined_on_incl.
 Qed.
 
 Inductive fstNoneOrR' {X Y:Type} (R:X->Y->Prop)
@@ -169,7 +246,7 @@ Proof.
   destruct if; eauto. subst. constructor; eauto. constructor.
 Qed.
 
-Lemma compile_typed DL AL ZL s ans_lv ans
+Lemma trs_srd DL AL ZL s ans_lv ans
   (RD:trs AL ZL s ans_lv ans)
   (LV:live_sound DL s ans_lv)
   (EQ:PIR2 lessReq AL DL)
